
\prob{004E}{三次方与三次方根}

求关于$x$的方程

\[ x^3 - \frac32\sqrt[3]6x^2 +3 = 0 \]

的实数根。
\problabels{yellow/代数, green/方程相关问题}

\ans{$x = \sqrt[3]6$或$x = -\sfrac12\sqrt[3]6$}

\subsection{因式分解}

基本思路：直接将等号左边因式分解求得其根。

将等号左边因式分解得

\begin{align*}
  & x^3 - \frac32\sqrt[3]6x^2 + 3 \\
  ={}& x^3 - 2\sqrt[3]6x^2 + \sqrt[3]6^2x + \frac12\sqrt[3]6x^2 - \sqrt[3]6^2x + 3 \\
  ={}& x\cdot x^2 - x\cdot 2\sqrt[3]6x + x\cdot\sqrt[3]6^2 \\
    &+ \frac12\sqrt[3]6\cdot x^2 - \frac12\sqrt[3]6\cdot2\sqrt[3]6x + \frac12\sqrt[3]6\cdot \sqrt[3]6^2 \\
  ={}& x\left(x^2 - 2\sqrt[3]6x + \sqrt[3]6^2\right) \\
  &+ \frac12\sqrt[3]6\left(x^2 - 2\sqrt[3]6x + \sqrt[3]6^2\right) \\
  ={}& \left(x + \frac12\sqrt[3]6\right)\left(x^2 - 2\sqrt[3]6x + \sqrt[3]6^2\right) \\
  ={}& \left(x + \frac12\sqrt[3]6\right)\left(x - \sqrt[3]6\right)^2 \\
\end{align*}

由于等号右边为0，故$x = \sqrt[3]6$或$x = -\sfrac12\sqrt[3]6$。

综上，原方程实数根为$x = \sqrt[3]6$或$x = -\sfrac12\sqrt[3]6$。
