
\prob{004F}{平方嵌套}

求关于$x$的方程

\[ (1 + x^2)^2 = 4x(1 - x^2) \]

的实数根。
\problabels{yellow/代数, green/方程相关问题}

\ans{$x = -1 \pm\sqrt2$}

\subsection{配方}

基本思路：将等式两边多次配方、降次后得出方程的根。

等式左边可变为

\begin{align*}
  (1 + x^2)^2 &= 1 + 2x^2 + (x^2)^2 \\
  &= 1 - 2x^2 + (x^2)^2 + 4x^2 \\
  &= (1 - x^2)^2 + 4x^2 \\
\end{align*}

故

\[ (1 - x^2)^2 + 4x^2 = 4x(1 - x^2) \]

移项得

\begin{align*}
  (1 - x^2)^2 + 4x^2 - 4x(1 - x^2) &= 0 \\
  (1 - x^2)^2 - 2\cdot2x(1 - x^2) + (2x)^2 &= 0 \\
  (1 - x^2 - 2x)^2 &= 0 \\
  -x^2 - 2x + 1 &= 0 \\
  x^2 - 2x - 1 &= 0 \\
\end{align*}

解一元二次方程得$x = -1 \pm\sqrt2$，故原方程实数根为$x = -1 \pm\sqrt2$。
