
\prob{0056}{六次多项式求值}

若$x = \sfrac1{\sqrt3 - \sqrt2}$，求

\[ x^6 - 2\sqrt2x^5 - x^4 + x^3 - 2\sqrt3x^2 + 2x - \sqrt2 \]

的值。
\problabels{yellow/代数, green/代数求值问题}

\ans{原式的值为$\sqrt3$。}

\subsection{化简中代入}

基本思路：在化简的过程中同时代入求值。

由$x = \sfrac1{\sqrt3 - \sqrt2}$易知

\begin{align*}
  x ={}& \frac{\sqrt3 + \sqrt2}{(\sqrt3 + \sqrt2)(\sqrt3 - \sqrt2)} \\
  ={}& \sqrt3 + \sqrt2 \\
  \text{原式} ={}& x^4\left(x^2 - 2\sqrt2x + 2\right) - 3x^4 \\
  &+ x\left(x^2 - 2\sqrt3x + 3\right) - x - \sqrt2 \\
  ={}& \left(\left(x - \sqrt2\right)^2 - 3\right)x^4 \\
  &+ \left(\left(x - \sqrt3\right)^2 - 1\right)x - \sqrt2 \\
\end{align*}

当$x = \sqrt3 + \sqrt2$时，

\begin{align*}
  \text{原式} &= (3 - 3)x^4 + (2 - 1)x - \sqrt2 \\
  &= x - \sqrt2 = \sqrt3 \\
\end{align*}

综上，原式的值为$\sqrt3$。
